Lectures 1 and 2

teaching/eutypes2018/code/state/Heap2.fsti
@@ -6,10 +6,10 @@ module Heap2
   val sel : #a:Type -> heap -> ref a -> GTot a
   val addr_of: #a:Type -> ref a -> GTot nat
 
-// BEGIN: modifies_contains
   val contains : #a:Type -> heap -> ref a -> Type0
 
-  let modifies (s:FStar.TSet.set nat) (h0 h1 : heap) : Type0 =
-    (forall (a:Type) (r:ref a).{:pattern (sel h1 r)}
-      (~(addr_of r `FStar.TSet.mem` s) /\ h0 `contains` r) ==> sel h1 r == sel h0 r)
+// BEGIN: modifies_contains
+  let modifies (s:FStar.TSet.set nat) (h0 h1 : heap) =
+    forall (a:Type) (r:ref a).{:pattern (sel h1 r)}
+        ~(addr_of r `FStar.TSet.mem` s) /\ h0 `contains` r ==> sel h1 r == sel h0 r
 // END: modifies_contains
